Bisimulations/LTS.lean
@@ -3,5 +3,3 @@ import Mathlib.Tactic.Lemma
 structure LTS (α : Type) where
   Node : Type
   transition : α → Node → Node → Prop
-
-def Rel (lts : LTS α) := lts.Node → lts.Node → Prop
